theories/L6_PCPS/closure_conversion_correct.v
@@ -2,10 +2,10 @@
  * Author: Zoe Paraskevopoulou, 2016
  *)
 
-Require Import L6.cps L6.cps_util L6.set_util L6.hoisting L6.identifiers L6.ctx L6.Ensembles_util
-        L6.List_util L6.functions L6.closure_conversion L6.eval L6.logical_relations.
+From L6 Require Import cps size_cps cps_util set_util hoisting identifiers ctx Ensembles_util
+        List_util functions closure_conversion eval logical_relations.
 Require Import Libraries.Coqlib.
-Require Import Coq.ZArith.Znumtheory Coq.Relations.Relations Coq.Arith.Wf_nat.
+Require Import Coq.ZArith.Znumtheory ArithRing Coq.Relations.Relations Coq.Arith.Wf_nat.
 Require Import Coq.Lists.List Coq.MSets.MSets Coq.MSets.MSetRBT Coq.Numbers.BinNums
         Coq.NArith.BinNat Coq.PArith.BinPos Coq.Sets.Ensembles Omega.
 
@@ -317,14 +317,14 @@ Section Closure_conversion_correct.
       intros B' H. eapply Hun. now constructor. 
     - rewrite <- app_ctx_f_fuse. intros B HB.
       rewrite project_vars_free_funs_in_exp in HB; [| eassumption ].
-      inv HB. inv H8.
+      inv HB. inv H9.
       + split; [| now apply Included_Empty_set ].
         eapply Included_trans.
         eapply Closure_conversion_occurs_free_Included_mut. eassumption.
         intros B HB. eapply Hun. inv HB; eauto.
         rewrite closure_conversion_fundefs_Same_set_image; [| eassumption ].
         rewrite Setminus_Same_set_Empty_set. now apply Included_Empty_set.
-      + rewrite make_closures_funs_in_exp in H9; [| eassumption ].
+      + rewrite make_closures_funs_in_exp in H10; [| eassumption ].
         eapply IHe; [ eassumption | | eassumption ].
         intros B1 HB1. eapply Hun. now constructor.
       + eapply IHB; [ eassumption | | eassumption ].
@@ -347,6 +347,100 @@ Section Closure_conversion_correct.
 
   (** ** Semantics preservation proof *)
 
+  (** We show observational approximation of the final results as well as an
+    * upper bound on the concrete execution cost of the translated program *)
+
+
+  (** *  Useful definitions and lemmas to express the upper bound. *)
+
+  Definition max_exp_env (k : nat) (e : exp) (rho : env) :=
+    max (sizeOf_exp e) (sizeOf_env k rho).
+
+  (* TODO move *)
+  
+  Lemma sizeOf_exp_grt_1 e :
+    1 <= sizeOf_exp e.
+  Proof.
+    induction e using exp_ind'; simpl; eauto; omega.
+  Qed.
+  
+  Lemma max_exp_env_grt_1 k e rho :
+    1 <= max_exp_env k e rho.
+  Proof.
+    unfold max_exp_env.
+    eapply le_trans. now apply sizeOf_exp_grt_1.
+    eapply Max.le_max_l.
+  Qed.
+
+  (** Lemmas used to establish the upper bound given the IH *)
+
+  Lemma max_exp_env_Econstr k x t ys e rho :
+    max_exp_env k e rho <= max_exp_env k (Econstr x t ys e) rho.
+  Proof.
+    eapply NPeano.Nat.max_le_compat_r.
+    simpl. omega.
+  Qed.
+
+  Lemma max_exp_env_Eproj k x t N y e rho :
+    max_exp_env k e rho <= max_exp_env k (Eproj x t N y e) rho.
+  Proof.
+    eapply NPeano.Nat.max_le_compat_r.
+    simpl. omega.
+  Qed.
+
+  Lemma max_exp_env_Ecase_cons_hd k x c e l rho :
+    max_exp_env k e rho <= max_exp_env k (Ecase x ((c, e) :: l)) rho.
+  Proof.
+    eapply NPeano.Nat.max_le_compat_r.
+    simpl. omega.
+  Qed.
+
+  Lemma max_exp_env_Ecase_cons_tl k x c e l rho :
+    max_exp_env k (Ecase x l) rho <= max_exp_env k (Ecase x ((c, e) :: l)) rho.
+  Proof.
+    eapply NPeano.Nat.max_le_compat_r.
+    simpl. omega.
+  Qed.
+
+  Lemma max_exp_env_Eprim k x f ys e rho :
+    max_exp_env k e rho <= max_exp_env k (Eprim x f ys e) rho.
+  Proof.
+    eapply NPeano.Nat.max_le_compat_r.
+    simpl. omega.
+  Qed.
+
+  Lemma max_exp_env_Efun k B e rho :
+    max_exp_env k e (def_funs B B rho rho) <= max_exp_env k (Efun B e) rho.
+  Proof.
+    unfold max_exp_env. eapply le_trans.
+    - eapply NPeano.Nat.max_le_compat_l.
+      now apply sizeOf_env_def_funs.
+    - rewrite (Max.max_comm (sizeOf_env _ _)), Max.max_assoc.
+      eapply NPeano.Nat.max_le_compat_r.
+      eapply Nat.max_lub; simpl; omega.
+  Qed.
+
+  (** * Definition of the bounds *)
+
+  (** Local predicate. Enforced only for the cost of the particular expressions
+    * related. It's likely that the upper bound can be refined further *)
+
+  Definition upper_boundL := 
+    fun i (e1 : exp) (rho1 : env) (c1 c2 : nat) =>
+      c2 <= 7 * c1 * (max_exp_env i e1 rho1) + 7 * sizeOf_exp e1.
+
+  Definition lower_boundL := 
+    fun (c1 c2 : nat) => c1 <= c2.
+  
+  Definition boundL (i : nat) (e1 : exp) (rho1 : env) (c1 : nat) (c2 : nat) : Prop :=
+    lower_boundL c1 c2 /\ upper_boundL i e1 rho1 c1 c2.
+  
+  (* Global predicate. Enforced on values.  *)
+  Definition boundG (k : nat) (p1 : exp * env * nat) (p2 : exp * env * nat) : Prop :=
+    let '(e1, rho1, c1) := p1 in
+    let '(e2, rho2, c2) := p2 in
+    boundL k e1 rho1 c1 c2.
+  
   (** Invariant about the values of free variables. *)
   Definition closure_env k rho Scope Funs vs FVs : Prop :=
     forall (x : var) N (v : val),
@@ -355,7 +449,7 @@ Section Closure_conversion_correct.
       nthN FVs N = Some x ->
       M.get x rho = Some v ->
       exists (v' : val),  nthN vs N = Some v' /\
-                     cc_approx_val pr cenv clo_tag k v v'.
+                     cc_approx_val pr cenv clo_tag k boundG v v'.
   
   (** Invariant about the free variables *) 
   Definition FV_inv k rho rho' Scope Funs c Γ FVs : Prop :=
@@ -367,7 +461,7 @@ Section Closure_conversion_correct.
       exists (vs : list val) (v' : val),
         M.get Γ rho' = Some (Vconstr c vs) /\
         nthN vs N = Some v' /\
-        cc_approx_val pr cenv clo_tag k v v'.
+        cc_approx_val pr cenv clo_tag k boundG v v'.
   
   (** Invariant about the functions in the current function definition *)
   Definition Fun_inv k (rho rho' : env) Scope Funs σ c Γ : Prop :=
@@ -380,7 +474,8 @@ Section Closure_conversion_correct.
         v = (Vfun rho1 B1 f1) /\
         ~ In _ Scope (σ f) /\
         M.get (σ f) rho' = Some (Vfun rho2 B2 f2) /\
-        cc_approx_val pr cenv clo_tag k (Vfun rho1 B1 f1)
+        cc_approx_val pr cenv clo_tag k boundG
+                      (Vfun rho1 B1 f1)
                       (Vconstr clo_tag [(Vfun rho2 B2 f2) ; (Vconstr c vs)]).
   
 
@@ -394,7 +489,7 @@ Section Closure_conversion_correct.
     ~ In _ Scope (σ f) ->
     ~ In _ (image σ (Setminus _ Funs Scope)) (σ f) ->
     M.get Γ rho' = Some (Vconstr c vs) ->
-    (cc_approx_val pr cenv clo_tag k (Vfun rho1 B1 f1)
+    (cc_approx_val pr cenv clo_tag k boundG (Vfun rho1 B1 f1)
                    (Vconstr clo_tag [(Vfun rho2 B2 f2) ; (Vconstr c vs)])) ->
     Fun_inv k (M.set f (Vfun rho1 B1 f1) rho)
             (M.set (σ f) (Vfun rho2 B2 f2) rho')
@@ -807,28 +902,41 @@ Section Closure_conversion_correct.
     - simpl; econstructor; eauto.
   Qed.
 
-  (** [(e1, ρ1) < (C [ e2 ], ρ2)] if [(e1, ρ1) < (e2, ρ2')], where [ρ2'] is the
-    interpretation of [C] in [ρ2] *)
-  Lemma ctx_to_rho_cc_approx_exp k rho1 rho2 rho2' C e e' :
-    ctx_to_rho C rho2 rho2' ->
-    cc_approx_exp pr cenv clo_tag k (e, rho1) (e', rho2') ->
-    cc_approx_exp pr cenv clo_tag k (e, rho1) (C |[ e' ]|, rho2).
-  Proof.  
-    intros Hctx Hcc. induction Hctx.
-    - assumption.
-    - intros v1 c1 Hleq1 Hstep1.
-      edestruct IHHctx as [v2 [c2 [Hstep2 Hcc2]]]; eauto.
-      repeat eexists; eauto.
-      simpl. econstructor; eauto.
-    - intros v1' c1 Hleq1 Hstep1.
-      edestruct IHHctx as [v2' [c2 [Hstep2 Hcc2]]]; eauto.
-      repeat eexists; eauto.
-      simpl. econstructor; eauto. simpl.
-      rewrite H, H0. reflexivity.
+  (* TODO move *)
+  Fixpoint sizeOf_exp_ctx (c : exp_ctx) : nat :=
+    match c with
+      | Hole_c => 0
+      | Econstr_c _ _ ys c => 1 + length ys + sizeOf_exp_ctx c
+      | Eproj_c _ _ _ _ c => 1 + sizeOf_exp_ctx c
+      | Eprim_c _ _ ys c => length ys + sizeOf_exp_ctx c
+      | Ecase_c _ l1 _ c l2  =>
+        1 + sizeOf_exp_ctx c
+        + fold_left (fun s p => s + sizeOf_exp (snd p)) l1 0
+        + fold_left (fun s p => s + sizeOf_exp (snd p)) l2 0 
+      | Efun1_c B c => sizeOf_fundefs B + sizeOf_exp_ctx c
+      | Efun2_c B e => sizeOf_fundefs_ctx B + sizeOf_exp e
+    end
+  with sizeOf_fundefs_ctx (B : fundefs_ctx) : nat :=
+         match B with
+           | Fcons1_c _ _ xs c B =>
+             1 + length xs + sizeOf_exp_ctx c + sizeOf_fundefs B
+           | Fcons2_c _ _ xs e B =>
+             1 + length xs + sizeOf_exp e + sizeOf_fundefs_ctx B
+         end.
+
+
+  (* TODO : move *)
+  Lemma inclusion_trans {A} P1 P2 P3 :
+    inclusion A P1 P2 ->
+    inclusion A P2 P3 ->
+    inclusion A P1 P3.
+  Proof.
+    now firstorder. 
   Qed.
 
-  (** * Various lemmas about [Closure_conversion_fundefs] *)
 
+  (** * Various lemmas about [Closure_conversion_fundefs] *)
+  
   Lemma closure_conversion_fundefs_find_def σ c Funs FVs B1 B2 f t1 xs e1 :
     injective_subdomain (name_in_fundefs B1) σ ->
     Closure_conversion_fundefs clo_tag Funs σ c FVs B1 B2 ->
@@ -1235,7 +1343,7 @@ Section Closure_conversion_correct.
        forall (e : exp) (rho rho' : env) (e' : exp)
          (Scope Funs : Ensemble var) σ c (Γ : var) (FVs : list var)
          (C : exp_ctx),
-         cc_approx_env_P pr cenv clo_tag Scope m rho rho' ->
+         cc_approx_env_P pr cenv clo_tag Scope m boundG rho rho' ->
          ~ In var (bound_var e) Γ ->
          binding_in_map (occurs_free e) rho ->
          fundefs_names_unique e ->
@@ -1244,7 +1352,7 @@ Section Closure_conversion_correct.
          Fun_inv m rho rho' Scope Funs σ c Γ ->
          FV_inv m rho rho' Scope Funs c Γ FVs ->
          Closure_conversion clo_tag Scope Funs σ c Γ FVs e e' C ->
-         cc_approx_exp pr cenv clo_tag m (e, rho) (C |[ e' ]|, rho')) ->
+         cc_approx_exp pr cenv clo_tag m (boundL m e rho) boundG (e, rho) (C |[ e' ]|, rho')) ->
     Same_set _ (occurs_free_fundefs B1) (FromList FVs) ->
     fundefs_names_unique_fundefs B1 ->
     fundefs_names_unique_fundefs B1' ->
@@ -1370,7 +1478,7 @@ Section Closure_conversion_correct.
   Lemma project_var_correct k rho1 rho2 rho2'
         Scope Funs σ c Γ FVs x x' C S S'  :
     project_var clo_tag Scope Funs σ c Γ FVs S x x' C S' ->
-    cc_approx_env_P pr cenv clo_tag Scope k rho1 rho2 ->
+    cc_approx_env_P pr cenv clo_tag Scope k boundG rho1 rho2 ->
     Fun_inv k rho1 rho2 Scope Funs σ c Γ ->
     FV_inv k rho1 rho2 Scope Funs c Γ FVs ->
     ctx_to_rho C rho2 rho2' ->
@@ -1378,10 +1486,10 @@ Section Closure_conversion_correct.
                         (Union var (image σ (Setminus _ Funs Scope))
                                (Union var (FromList FVs) (Singleton var Γ)))) ->
     ~ In _ S' x' /\
-    cc_approx_env_P pr cenv clo_tag Scope k rho1 rho2' /\
+    cc_approx_env_P pr cenv clo_tag Scope k boundG rho1 rho2' /\
     Fun_inv k rho1 rho2' Scope Funs σ c Γ /\
     FV_inv k rho1 rho2' Scope Funs c Γ FVs /\
-    cc_approx_var_env pr cenv clo_tag k rho1 rho2' x x'.
+    cc_approx_var_env pr cenv clo_tag k boundG rho1 rho2' x x'.
   Proof.
     intros Hproj Hcc Hfun Henv Hctx Hd.
     inv Hproj.
@@ -1427,25 +1535,25 @@ Section Closure_conversion_correct.
         rewrite Hget' in H10; inv H10.
         rewrite H11 in Hnth. now inv Hnth.
   Qed.
-
+  
   (** Correctness of [project_vars] *)
   Lemma project_vars_correct k rho1 rho2 rho2'
         Scope Funs σ c Γ FVs xs xs' C S S' :
     project_vars clo_tag Scope Funs σ c Γ FVs S xs xs' C S' ->
-    cc_approx_env_P pr cenv clo_tag Scope k rho1 rho2 ->
+    cc_approx_env_P pr cenv clo_tag Scope k boundG rho1 rho2 ->
     Fun_inv k rho1 rho2 Scope Funs σ c Γ ->
     FV_inv k rho1 rho2 Scope Funs c Γ FVs ->
     ctx_to_rho C rho2 rho2' ->
     Disjoint _ S (Union var Scope
                         (Union var (image σ (Setminus _ Funs Scope))
                                (Union var (FromList FVs) (Singleton var Γ)))) ->
-    cc_approx_env_P pr cenv clo_tag Scope k rho1 rho2' /\
+    cc_approx_env_P pr cenv clo_tag Scope k boundG rho1 rho2' /\
     Fun_inv k rho1 rho2' Scope Funs σ c Γ /\
     FV_inv k rho1 rho2' Scope Funs c Γ FVs /\
     (forall vs,
        getlist xs rho1 = Some vs ->
        exists vs', getlist xs' rho2' = Some vs' /\
-              Forall2 (cc_approx_val pr cenv clo_tag k) vs vs').
+              Forall2 (cc_approx_val pr cenv clo_tag k boundG) vs vs').
   Proof.
     revert k rho1 rho2 rho2' Scope Funs Γ FVs xs' C S.
     induction xs;
@@ -1469,6 +1577,7 @@ Section Closure_conversion_correct.
       eexists. split; eauto. simpl. rewrite Hgetlist'. 
       erewrite <- project_vars_get; eauto. rewrite Hget'''. reflexivity.
   Qed.
+  
 
   (** Correctness of [make_closures] *)
   Lemma make_closures_correct k rho1 rho2 rho2' B S c' Γ' C σ S' σ' Scope Funs FVs c Γ :
@@ -1478,12 +1587,12 @@ Section Closure_conversion_correct.
     ~ In _ (name_in_fundefs B) Γ' ->
     Included _ (name_in_fundefs B) Scope ->
     Disjoint _ S (name_in_fundefs B) ->
-    cc_approx_env_P pr cenv clo_tag (Setminus _ Scope (name_in_fundefs B)) k rho1 rho2 ->
+    cc_approx_env_P pr cenv clo_tag (Setminus _ Scope (name_in_fundefs B)) k boundG rho1 rho2 ->
     Fun_inv k rho1 rho2 Scope Funs σ' c Γ ->  
     FV_inv k rho1 rho2 Scope Funs c Γ FVs ->
     Fun_inv k rho1 rho2 (Empty_set _) (name_in_fundefs B) σ c' Γ' ->
     ctx_to_rho C rho2 rho2' ->
-    cc_approx_env_P pr cenv clo_tag Scope k rho1 rho2' /\
+    cc_approx_env_P pr cenv clo_tag Scope k boundG rho1 rho2' /\
     Fun_inv k rho1 rho2' Scope Funs σ' c Γ /\
     FV_inv k rho1 rho2' Scope Funs c Γ FVs.
   Proof.
@@ -1491,9 +1600,8 @@ Section Closure_conversion_correct.
     induction Hmake;
       intros k rho1 rho2 rho2' Scope Funs FVs Γ1 Hun Hnin1 Hnin2
              Hsub Hd Hcc Hfun Henv Hfun' Hctx.
-    - inv Hctx. repeat split; eauto.
-      simpl in *.
-      rewrite Setminus_Empty_set_neut_r in Hcc. eassumption.
+    - inv Hctx. repeat split; eauto. rewrite Setminus_Empty_set_neut_r in Hcc.
+      eassumption.
     - eapply ctx_to_rho_comp_ctx_l in Hctx; [| apply Constr_cc; constructor ].
       destruct Hctx as [rho2'' [Hctx1 Hctx2]].
       inv Hctx1. inv H10. inv Hun.
@@ -1540,10 +1648,566 @@ Section Closure_conversion_correct.
       + eauto.
   Qed.
 
+
+
+  (** Properties about context sizes *)
+
+  Lemma project_var_sizeOf_ctx_exp (Scope Funs : Ensemble var) (σ : var -> var) 
+    (c : cTag) (Γ : var) (FVs : list var) (S : Ensemble var) 
+    (x x' : var) (C : exp_ctx) (S' : Ensemble var) :
+    project_var clo_tag Scope Funs σ c Γ FVs S x x' C S' ->
+    sizeOf_exp_ctx C <= 3. 
+  Proof.
+    intros Hctx. inv Hctx; eauto.
+  Qed.
+
+  (* TODO move *)
+  Lemma sizeOf_exp_ctx_comp_ctx_mut :
+    (forall C1 C2,
+       sizeOf_exp_ctx (comp_ctx_f C1 C2) = sizeOf_exp_ctx C1 + sizeOf_exp_ctx C2) /\
+    (forall B e,
+       sizeOf_fundefs_ctx (comp_f_ctx_f B e) = sizeOf_fundefs_ctx B + sizeOf_exp_ctx e).
+  Proof.
+    exp_fundefs_ctx_induction IHe IHB; 
+    try (intros C; simpl; eauto; rewrite IHe; omega);
+    try (intros C; simpl; eauto; rewrite IHB; omega).
+    (* probably tactic misses an intro pattern *)
+    intros l' C. simpl. rewrite IHe; omega.
+  Qed.
+
+  Corollary sizeOf_exp_ctx_comp_ctx :
+    forall C1 C2,
+      sizeOf_exp_ctx (comp_ctx_f C1 C2) = sizeOf_exp_ctx C1 + sizeOf_exp_ctx C2.
+  Proof.
+    eapply sizeOf_exp_ctx_comp_ctx_mut; eauto.
+  Qed.
+
+  Corollary sizeOf_fundefs_ctx_comp_f_ctx :
+    forall B e,
+      sizeOf_fundefs_ctx (comp_f_ctx_f B e) = sizeOf_fundefs_ctx B + sizeOf_exp_ctx e.
+  Proof.
+    eapply sizeOf_exp_ctx_comp_ctx_mut; eauto.
+  Qed.
+
+  
+  Lemma project_vars_sizeOf_ctx_exp (Scope Funs : Ensemble var) (σ : var -> var) 
+    (c : cTag) (Γ : var) (FVs : list var) (S : Ensemble var) 
+    (xs xs' : list var) (C : exp_ctx) (S' : Ensemble var)  :
+    project_vars clo_tag Scope Funs σ c Γ FVs S xs xs' C S' ->
+    sizeOf_exp_ctx C <= 3 * length xs. 
+  Proof.
+    intros Hctx. induction Hctx; eauto.
+    rewrite sizeOf_exp_ctx_comp_ctx. simpl.
+    specialize (project_var_sizeOf_ctx_exp _ _ _ _ _ _ _ _ _ _ _ H).
+    omega.
+  Qed.
+
+  Lemma make_closures_sizeOf_ctx_exp (B : fundefs) (S : Ensemble var) (Γ : var)
+        (C : exp_ctx) (σ : var -> var) (S' : Ensemble var) :
+    make_closures clo_tag B S Γ C σ S' ->
+    sizeOf_exp_ctx C <= 3 * numOf_fundefs B.
+  Proof.
+    induction 1; eauto.
+    simpl. specialize (sizeOf_exp_grt_1 e).
+    omega.
+  Qed.
+  
+  (* TODO move *)
+
+  Lemma cc_approx_val_cc_appox_var_env k P rho1 rho2 x y v1 v2 :
+    M.get x rho1 = Some v1 -> M.get y rho2 = Some v2 ->
+    cc_approx_val pr cenv clo_tag k P v1 v2 ->
+    cc_approx_var_env pr cenv clo_tag k P rho1 rho2 x y.
+  Proof.
+    intros Hget1 Hget2 Hcc.
+    intros v1' Hget1'. rewrite Hget1 in Hget1'. inv Hget1'.
+    firstorder.
+  Qed.
+
+  Lemma Forall2_cc_approx_var_env k P rho1 rho2 l1 l2 vs1 vs2 :
+    getlist l1 rho1 = Some vs1 ->
+    getlist l2 rho2 = Some vs2 ->
+    Forall2 (cc_approx_val pr cenv clo_tag k P) vs1 vs2 ->
+    Forall2 (cc_approx_var_env pr cenv clo_tag k P rho1 rho2) l1 l2.
+  Proof.
+    revert vs1 l2 vs2; induction l1; intros vs1 l2 vs2  Hget1 Hget2 Hall.
+    - destruct vs1; try discriminate.
+      inv Hall. destruct l2; try discriminate.
+      now constructor.
+      simpl in Hget2. destruct (M.get e rho2); try discriminate.
+      destruct (getlist l2 rho2); try discriminate.
+    - simpl in Hget1.
+      destruct (M.get a rho1) eqn:Hgeta; try discriminate.
+      destruct (getlist l1 rho1) eqn:Hgetl; try discriminate.
+      inv Hget1.
+      inv Hall.
+      destruct l2; try discriminate. simpl in Hget2.
+      destruct (M.get e rho2) eqn:Hgeta'; try discriminate.
+      destruct (getlist l2 rho2) eqn:Hgetl'; try discriminate.
+      inv Hget2. constructor; eauto.
+      eapply cc_approx_val_cc_appox_var_env; eauto.
+  Qed.
+
+  (** [(e1, ρ1) < (C [ e2 ], ρ2)] if [(e1, ρ1) < (e2, ρ2')], where [ρ2'] is the
+      interpretation of [C] in [ρ2] *)
+  Lemma ctx_to_rho_cc_approx_exp k (P : nat -> relation nat) P' rho1 rho2 rho2' C e e' :
+    inclusion _ P' (P 0) ->
+    (forall c1 c2 n c ,  P n c1 c2 -> P (n + c) c1 (c2 + c)) ->
+    ctx_to_rho C rho2 rho2' -> 
+    cc_approx_exp pr cenv clo_tag k P' boundG (e, rho1) (e', rho2') ->
+    cc_approx_exp pr cenv clo_tag k (P (sizeOf_exp_ctx C)) boundG (e, rho1) (C |[ e' ]|, rho2).
+  Proof.  
+    intros H1 H2 Hctx Hcc. induction Hctx.
+    - intros v1' c1 Hleq1 Hstep1.
+      edestruct Hcc as [v2' [c2 [Hstep2 [Hub Hcc2]]]]; try eassumption.
+      firstorder.
+    - intros v1 c1 Hleq1 Hstep1.
+      edestruct IHHctx as [v2 [c2 [Hstep2 [HP Hcc2]]]]; try eassumption.
+      repeat eexists.
+      now econstructor; eauto.
+      simpl.
+      rewrite (plus_comm 1). now eauto.
+      eassumption.
+    - intros v1' c1 Hleq1 Hstep1.
+      edestruct IHHctx as [v2' [c2 [Hstep2 [Hub Hcc2]]]]; try eassumption.
+      repeat eexists.
+      simpl. econstructor; eauto. simpl.
+      rewrite H, H0. reflexivity.
+      simpl. do 3 rewrite (plus_comm 1). 
+      rewrite !plus_assoc_reverse. simpl. now eauto.
+      eassumption.
+  Qed.
+  
+  Lemma cc_approx_exp_ctx_to_rho k (P' : nat -> relation nat) P rho1 rho2 rho2' C e e' :
+    inclusion _ (P' 0) P ->
+    (forall c1 c2 c n, c <= sizeOf_exp_ctx C -> P' (n + c) c1 (c2 + c) -> P' n c1 c2) ->
+    ctx_to_rho C rho2 rho2' -> 
+    cc_approx_exp pr cenv clo_tag k (P' (sizeOf_exp_ctx C)) boundG (e, rho1) (C |[ e' ]|, rho2) ->
+    cc_approx_exp pr cenv clo_tag k P boundG (e, rho1) (e', rho2').
+  Proof.  
+    intros H1 H2 Hctx Hcc. induction Hctx.
+    - intros v1' c1 Hleq1 Hstep1.
+      edestruct Hcc as [v2' [c2 [Hstep2 [Hub Hcc2]]]]; try eassumption.
+      firstorder.
+    - eapply IHHctx; eauto.
+      + intros c1 c2 c3 n Hleq. eapply H2. simpl; omega.
+      + intros v1 c1 Hleq1 Hstep1.
+        edestruct Hcc as [v2 [c2 [Hstep2 [Hub Hcc2]]]]; try eassumption.
+        inv Hstep2. rewrite H in H11; inv H11. rewrite H12 in H0; inv H0.
+        repeat eexists; eauto.
+        simpl in Hub. rewrite (plus_comm 1) in Hub. eapply H2; try eassumption.
+        simpl; omega.
+    - eapply IHHctx; eauto.
+      intros c1 c2 c3 n Hleq. eapply H2; simpl; omega.
+      intros v1' c1' Hleq1 Hstep1.
+      edestruct Hcc as [v2' [c2' [Hstep2 [Hub Hcc2]]]]; try eassumption.
+      inv Hstep2. simpl in H10. rewrite H, H0 in H10. inv H10.
+      repeat eexists; eauto.
+      simpl in Hub. do 3 rewrite (plus_comm 1) in Hub. 
+      rewrite !plus_assoc_reverse in Hub. eapply H2; try eassumption.
+      simpl; omega.
+  Qed.
+
+  Lemma mult_le_n n m :
+    1 <= m ->
+    n <= n * m.
+  Proof.
+    rewrite Nat.mul_comm.
+    edestruct mult_O_le; eauto. omega.
+  Qed.
+
+  Lemma plus_le_mult  (a1 a2 b1 b2 b3 : nat) :
+    b3 <= a1 ->
+    1 <= b2 ->
+    a2 <= b1 * b3 ->
+    a1 + a2 <= (1 + b1) * a1 * b2.
+  Proof.
+    intros.
+    rewrite <- mult_assoc, NPeano.Nat.mul_add_distr_r.
+    eapply plus_le_compat.
+    - simpl. rewrite <- plus_n_O.
+      now eapply mult_le_n.
+    - eapply le_trans. eapply le_trans. eassumption.
+      eapply mult_le_compat. eauto. eassumption.
+      rewrite mult_assoc. eapply mult_le_n. eassumption.
+  Qed.      
+  
+  Lemma Ecase_correct_upper_bound k rho1 rho2 rho2' C x x' c e e' l l' :
+    ctx_to_rho C rho2 rho2' ->
+    sizeOf_exp_ctx C <= 3 ->
+    Forall2 (fun p1 p2 : cTag * exp => fst p1 = fst p2) l l' ->
+    cc_approx_var_env pr cenv clo_tag k boundG rho1 rho2' x x' ->
+    cc_approx_exp pr cenv clo_tag k (upper_boundL k e rho1)
+                  boundG (e, rho1) (e', rho2') ->
+    cc_approx_exp pr cenv clo_tag k (upper_boundL k (Ecase x l) rho1)
+                  boundG (Ecase x l, rho1) (C |[ Ecase x' l' ]|, rho2) ->
+    cc_approx_exp pr cenv clo_tag k (upper_boundL k (Ecase x ((c, e) :: l)) rho1)
+                  boundG (Ecase x ((c, e) :: l), rho1)
+                  (C |[ Ecase x' ((c, e') :: l') ]|, rho2).
+  Proof.
+    intros Hctx Hleq Hall Henv Hcc1 Hcc2.
+    eapply cc_approx_exp_rel_mon.
+    pose (rhs := fun (n : nat) c1 =>
+                   (7 * c1 * max_exp_env k (Ecase x ((c, e) :: l)) rho1 + n) + 7 * sizeOf_exp (Ecase x ((c, e) :: l))).
+    { eapply ctx_to_rho_cc_approx_exp with
+      (P := fun n c1 c2 => c2 + sizeOf_exp_ctx C <= rhs n c1)
+        (P' := fun c1 c2 => c2 + sizeOf_exp_ctx C <= rhs 0 c1); try eassumption.
+      - intros n1 n2. unfold rhs.  omega.
+      - unfold rhs. intros c1 c2 n' c' H. omega.
+      - eapply cc_approx_exp_case_cons_compat 
+        with (S' := fun c1 c2 => c2 + sizeOf_exp_ctx C <=
+                              7 * c1 * max_exp_env k (Ecase x l) rho1
+                              + 7 * sizeOf_exp (Ecase x l)); try eassumption.
+        + intros c1 c2 c' Hle. unfold upper_boundL, rhs. intros H.
+          eapply le_trans with (m := 7 * c1 * max_exp_env k e rho1 + c' + 3
+                                     + 7 * sizeOf_exp e).
+          * omega.
+          * rewrite <- plus_n_O. eapply plus_le_compat; [| simpl; omega ]. 
+            ring_simplify. rewrite <- plus_assoc.
+            eapply plus_le_compat. eapply mult_le_compat. eauto.
+            now apply max_exp_env_Ecase_cons_hd.
+            replace 7 with (1 + 6) by omega.
+            eapply plus_le_mult; eauto.
+            now eapply max_exp_env_grt_1. omega.
+        + intros c1 c2 c' Hle. unfold rhs. intros H. ring_simplify.
+          rewrite <- (plus_assoc _ _ (7 * _)).
+          rewrite (plus_comm _ c'), <- plus_assoc. eapply plus_le_compat.
+          * rewrite (mult_comm _ c'), <- mult_assoc.
+            eapply mult_le_n. rewrite <- (Nat.mul_1_r 1).
+            eapply NPeano.Nat.mul_le_mono. omega.
+            now eapply max_exp_env_grt_1.
+          * eapply le_trans; eauto.
+            eapply plus_le_compat; [| simpl; omega ].
+            eapply mult_le_compat; eauto. now apply max_exp_env_Ecase_cons_tl.
+        + eapply cc_approx_exp_ctx_to_rho with
+          (P' := fun n c1 c2 => c2 + sizeOf_exp_ctx C <=
+                             7 * c1 * max_exp_env k (Ecase x l) rho1 +
+                             7 * sizeOf_exp (Ecase x l)+ n); try eassumption.
+          * intros n1 n2 H. omega.
+          * intros c1 c2 c3 n Hlt. omega.
+          * eapply cc_approx_exp_rel_mon. eassumption.
+            intros n1 n2. unfold upper_boundL. omega. }
+    intros c1 c2 H. unfold upper_boundL. omega. 
+  Qed.
+
+  Lemma Ecase_correct_lower_bound k rho1 rho2 rho2' C x x' c e e' l l' :
+    ctx_to_rho C rho2 rho2' ->
+    sizeOf_exp_ctx C <= 3 ->
+    Forall2 (fun p1 p2 : cTag * exp => fst p1 = fst p2) l l' ->
+    cc_approx_var_env pr cenv clo_tag k boundG rho1 rho2' x x' ->
+    cc_approx_exp pr cenv clo_tag k lower_boundL
+                  boundG (e, rho1) (e', rho2') ->
+    cc_approx_exp pr cenv clo_tag k lower_boundL
+                  boundG (Ecase x l, rho1) (C |[ Ecase x' l' ]|, rho2) ->
+    cc_approx_exp pr cenv clo_tag k lower_boundL
+                  boundG (Ecase x ((c, e) :: l), rho1)
+                  (C |[ Ecase x' ((c, e') :: l') ]|, rho2).
+  Proof.
+    intros Hctx Hleq Hall Henv Hcc1 Hcc2.
+    eapply cc_approx_exp_rel_mon.
+    eapply ctx_to_rho_cc_approx_exp
+    with (P := fun n c1 c2 => c1 + n <= c2 + sizeOf_exp_ctx C)
+      (P' := fun c1 c2 => c1 <= c2 + sizeOf_exp_ctx C); try eassumption.
+    - intros n c1 c2. simpl. omega.
+    - intros c1 c2 n' c'. simpl. omega.
+    - eapply cc_approx_exp_case_cons_compat
+      with (S' := fun c1 c2 : nat => c1 <= c2 + sizeOf_exp_ctx C); try eassumption.
+      + intros c1 c2 c'. unfold lower_boundL. simpl. omega.
+        + intros c1 c2 c'. simpl. omega.
+        + eapply cc_approx_exp_ctx_to_rho with
+          (P' := fun n c1 c2 => c1 + n <= c2 + sizeOf_exp_ctx C); try eassumption.
+          * intros c1 c2. simpl. omega.
+          * intros c1 c2 c3 n Hlt. omega.
+          * eapply cc_approx_exp_rel_mon. eassumption. intros c1 c2. unfold lower_boundL. omega.
+    - intros c1 c2 c'. unfold lower_boundL. simpl. omega.
+  Qed.
+
+  Lemma Union_Included_l {A} S1 S2 S3 :
+    Union A S1 S2 \subset S3 ->
+    S1 \subset S3.
+  Proof.
+    firstorder.
+  Qed.
+
+  Lemma Union_Included_r {A} S1 S2 S3 :
+    Union A S1 S2 \subset S3 ->
+    S2 \subset S3.
+  Proof.
+    firstorder.
+  Qed.
+
+  Lemma FromList_subset_included {A} (l1 l2 : list A) :
+    FromList l1 \subset FromList l2 <->
+    incl l1 l2.
+  Proof.
+    split; eauto.
+  Qed.  
+  
+  Lemma Same_set_FromList_length {A} (l1 l2 : list A) :
+    NoDup l1 ->
+    FromList l1 \subset FromList l2 ->
+    length l1 <= length l2.
+  Proof.
+    eapply NoDup_incl_length.
+  Qed.
+
+  Lemma Singleton_Included_r {A : Type} (x : A) (S : Ensemble A) :
+    [set x] \subset S -> In A S x.
+  Proof.
+    firstorder.
+  Qed.
+
+  Require Import Coq.Sorting.Permutation.
+
+  Lemma FromList_Union_split {A} (l : list A) S1 S2 :
+    FromList l \subset Union _ S1 S2 ->
+    exists l1 l2,
+      Permutation (l1 ++ l2) l /\
+      FromList l1 \subset S1 /\
+      FromList l2 \subset S2.
+  Proof.
+    induction l; intros Hun.
+    - exists [], []. firstorder.
+    - rewrite FromList_cons in Hun.
+      assert (Hin1 := Union_Included_l _ _ _ Hun).
+      assert (Hin2 := Union_Included_r _ _ _ Hun).      
+      eapply Singleton_Included_r in Hin1.
+      edestruct IHl as [l1 [l2 [Hperm [Hs1 Hs2]]]]; eauto.
+      inv Hin1.
+      + eexists (a :: l1), l2. 
+        split; [| split ].
+        rewrite <- app_comm_cons. eapply perm_skip.
+        eassumption.
+        rewrite FromList_cons. eapply Union_Included; eauto.
+        eapply Singleton_Included. eauto.
+        eassumption.
+      + eexists l1, (a :: l2). 
+        split; [| split ].
+        rewrite Permutation_app_comm.
+        rewrite <- app_comm_cons. eapply perm_skip.
+        rewrite <- Permutation_app_comm. eassumption.
+        eassumption.
+        rewrite FromList_cons. eapply Union_Included; eauto.
+        eapply Singleton_Included. eauto.
+  Qed.
+
+  Lemma NoDup_cons_l {A} (l1 l2 : list A):
+    NoDup (l1 ++ l2) ->
+    NoDup l1.
+  Proof.
+    induction l1; simpl; intros H; constructor; eauto.
+    - inv H. firstorder.
+    - inv H; firstorder.
+  Qed.
+
+  Lemma NoDup_cons_r {A} (l1 l2 : list A):
+    NoDup (l1 ++ l2) ->
+    NoDup l2.
+  Proof.
+    revert l2; induction l1; intros l2 H; simpl in *; eauto.
+    inv H; eauto.
+  Qed.
+
+  Lemma In_occurs_free_Ecase x l :
+    x \in occurs_free (Ecase x l).
+  Proof.
+    firstorder.
+  Qed.
+    
+  (* TODO move *)
+  Lemma occurs_free_cardinality_mut :
+    (forall e FVs,
+       FromList FVs \subset occurs_free e ->
+       NoDup FVs ->
+       length FVs <= sizeOf_exp e) /\
+    (forall B FVs,
+       FromList FVs \subset occurs_free_fundefs B ->
+       NoDup FVs ->
+       length FVs <= sizeOf_fundefs B).
+  Proof.
+    exp_defs_induction IHe IHl IHb; intros FVs Heq Hnd;
+    try repeat normalize_occurs_free_in_ctx; simpl.
+    - edestruct (@FromList_Union_split var) as [l1 [l2 [HP [Hin1 Hin2]]]].
+      eassumption.
+      rewrite <- HP in Hnd.
+      eapply Permutation_length in HP. rewrite <- HP.
+      rewrite app_length.
+      eapply (Included_trans (FromList l2) (Setminus var (occurs_free e) [set v])) in Hin2;
+      [| now apply Setminus_Included ].
+      eapply Same_set_FromList_length in Hin1.
+      eapply IHe in Hin2. omega.
+      eapply NoDup_cons_r; eauto. 
+      eapply NoDup_cons_l; eauto.
+    - rewrite <- (Union_Empty_set_neut_r [set v]) in Heq.
+      rewrite <- FromList_nil, <- FromList_cons in Heq.
+      eapply Same_set_FromList_length in Heq; eauto.
+    - rewrite Union_commut, <- Union_assoc, (Union_commut (occurs_free (Ecase v l))),
+      (Union_Same_set [set v]) in Heq.
+      edestruct (@FromList_Union_split var) as [l1 [l2 [HP [Hin1 Hin2]]]].
+      eassumption.
+      rewrite <- HP in Hnd.
+      eapply Permutation_length in HP. rewrite <- HP.
+      rewrite !app_length.
+      eapply IHe in Hin1. eapply IHl in Hin2. simpl in *. omega.
+      eapply NoDup_cons_r; eauto. 
+      eapply NoDup_cons_l; eauto.
+      eapply Singleton_Included. eauto.
+    - edestruct (@FromList_Union_split var) as [l1 [l2 [HP [Hin1 Hin2]]]].
+      eassumption.
+      rewrite <- HP in Hnd.
+      eapply Permutation_length in HP. rewrite <- HP.
+      rewrite app_length.
+      eapply (Included_trans (FromList l2) (Setminus var (occurs_free e) [set v])) in Hin2;
+        [| now apply Setminus_Included ].
+      rewrite <- (Union_Empty_set_neut_r [set v0]) in Hin1.
+      rewrite <- FromList_nil, <- FromList_cons in Hin1.
+      eapply Same_set_FromList_length in Hin1.
+      eapply IHe in Hin2. simpl in *. omega.
+      eapply NoDup_cons_r; eauto. 
+      eapply NoDup_cons_l; eauto.
+    - edestruct (@FromList_Union_split var) as [l1 [l2 [HP [Hin1 Hin2]]]].
+      eassumption.
+      rewrite <- HP in Hnd.
+      eapply Permutation_length in HP. rewrite <- HP.
+      rewrite app_length.
+      eapply (Included_trans (FromList l2) (Setminus var (occurs_free e) _)) in Hin2;
+        [| now apply Setminus_Included ].
+      eapply IHb in Hin1. eapply IHe in Hin2. omega.
+      eapply NoDup_cons_r; eauto. 
+      eapply NoDup_cons_l; eauto.
+    - edestruct (@FromList_Union_split var) as [l1 [l2 [HP [Hin1 Hin2]]]].
+      eassumption. rewrite <- HP in Hnd.
+      eapply Same_set_FromList_length in Hin1; eauto.
+      eapply Permutation_length in HP. rewrite <- HP.
+      rewrite app_length.
+      rewrite <- (Union_Empty_set_neut_r [set v]) in Hin2.
+      rewrite <- FromList_nil, <- FromList_cons in Hin2.
+      eapply Same_set_FromList_length in Hin2.
+      simpl in *. omega.
+      eapply NoDup_cons_r; eauto. 
+      eapply NoDup_cons_l; eauto.
+    - edestruct (@FromList_Union_split var) as [l1 [l2 [HP [Hin1 Hin2]]]].
+      eassumption.
+      rewrite <- HP in Hnd.
+      eapply Permutation_length in HP. rewrite <- HP.
+      rewrite app_length.
+      eapply (Included_trans (FromList l2) (Setminus var (occurs_free e) [set v])) in Hin2;
+      [| now apply Setminus_Included ].
+      eapply Same_set_FromList_length in Hin1.
+      eapply IHe in Hin2. omega.
+      eapply NoDup_cons_r; eauto. 
+      eapply NoDup_cons_l; eauto.
+    - rewrite occurs_free_Ehalt in Heq.
+      rewrite <- (Union_Empty_set_neut_r [set v]) in Heq.
+      rewrite <- FromList_nil, <- FromList_cons in Heq.
+      eapply Same_set_FromList_length in Heq; eauto.
+    - edestruct (@FromList_Union_split var) as [l1 [l2 [HP [Hin1 Hin2]]]].
+      eassumption. rewrite <- HP in Hnd.
+      eapply Permutation_length in HP. rewrite <- HP.
+      rewrite app_length.
+      eapply (Included_trans (FromList l2) (Setminus var _ [set v])) in Hin2;
+         [| now apply Setminus_Included ].
+      eapply (Included_trans (FromList l1) (Setminus var _ _)) in Hin1;
+        [| now apply Setminus_Included ]. 
+      eapply IHe in Hin1. eapply IHb in Hin2. omega.
+      eapply NoDup_cons_r; eauto. 
+      eapply NoDup_cons_l; eauto.
+    - rewrite <- FromList_nil in Heq.
+      apply Same_set_FromList_length in Heq; eauto.
+  Qed.
+
+  Corollary occurs_free_cardinality :
+    (forall e FVs,
+       FromList FVs \subset occurs_free e ->
+       NoDup FVs ->
+       length FVs <= sizeOf_exp e).
+  Proof.
+    eapply occurs_free_cardinality_mut.
+  Qed.
+
+  Corollary occurs_free_fundefs_cardinality :
+    (forall B FVs,
+       FromList FVs \subset occurs_free_fundefs B ->
+       NoDup FVs ->
+       length FVs <= sizeOf_fundefs B).
+  Proof.
+    eapply occurs_free_cardinality_mut.
+  Qed.
+  
+  (* TODO move *)
+  Lemma cc_approx_exp_rel_conj k P1 P2 P rho1 rho2 e1 e2 :
+    cc_approx_exp pr cenv clo_tag k P1 P (e1, rho1) (e2, rho2) ->
+    cc_approx_exp pr cenv clo_tag k P2 P (e1, rho1) (e2, rho2) ->
+    cc_approx_exp pr cenv clo_tag k (fun c1 c2 => P1 c1 c2 /\ P2 c1 c2) P (e1, rho1) (e2, rho2).
+  Proof. 
+    intros Hcc1 Hcc2 v c Hlt Hstep.
+    edestruct Hcc1 as [v1 [c1 [Hstep1 [HP1 Hv1]]]]; eauto.
+    edestruct Hcc2 as [v2 [c2 [Hstep2 [HP2 Hv2]]]]; eauto.
+    eapply bstep_cost_deterministic in Hstep1; eauto. inv Hstep1.
+    firstorder.
+  Qed.
+
+  Opaque mult.
+
+  Corollary Ecase_correct k rho1 rho2 rho2' C x x' c e e' l l' :
+    ctx_to_rho C rho2 rho2' ->
+    sizeOf_exp_ctx C <= 3 ->
+    Forall2 (fun p1 p2 : cTag * exp => fst p1 = fst p2) l l' ->
+    cc_approx_var_env pr cenv clo_tag k boundG rho1 rho2' x x' ->
+    cc_approx_exp pr cenv clo_tag k (boundL k e rho1)
+                  boundG (e, rho1) (e', rho2') ->
+    cc_approx_exp pr cenv clo_tag k (boundL k (Ecase x l) rho1)
+                  boundG (Ecase x l, rho1) (C |[ Ecase x' l' ]|, rho2) ->
+    cc_approx_exp pr cenv clo_tag k (boundL k (Ecase x ((c, e) :: l)) rho1)
+                  boundG (Ecase x ((c, e) :: l), rho1)
+                  (C |[ Ecase x' ((c, e') :: l') ]|, rho2).
+  Proof.
+    intros. eapply cc_approx_exp_rel_conj.
+    eapply Ecase_correct_lower_bound; eauto.
+    eapply cc_approx_exp_rel_mon; eauto. now firstorder.
+    eapply cc_approx_exp_rel_mon; eauto. now firstorder.
+    eapply Ecase_correct_upper_bound; eauto.
+    eapply cc_approx_exp_rel_mon; eauto. now firstorder.
+    eapply cc_approx_exp_rel_mon; eauto. now firstorder.
+  Qed.
+
+  Lemma Closure_conversion_fundefs_numOf_fundefs (Funs : Ensemble var) (σ : var -> var) (c : cTag) 
+        (FVs : list var) (B1 B2 : fundefs) :
+    Closure_conversion_fundefs clo_tag Funs σ c FVs B1 B2 ->
+    numOf_fundefs B1 = numOf_fundefs B2.
+  Proof.
+    intros Hcc; induction Hcc; eauto; simpl. congruence.
+  Qed.
+
+  Lemma fun_in_fundefs_sizeOf_exp B f tau xs e :
+    fun_in_fundefs B (f, tau, xs, e) ->
+    sizeOf_exp e <= sizeOf_fundefs B.
+  Proof.
+    intros Hin. induction B; inv Hin.
+    - inv H. simpl; omega.
+    - eapply le_trans. eapply IHB; eauto.
+      simpl. omega.
+  Qed.
+
+  Lemma sizeOf_env_O rho :
+    sizeOf_env 0 rho = 0.
+  Proof.
+    unfold sizeOf_env, max_ptree_with_measure.
+    rewrite M.fold_spec. generalize (M.elements rho).
+    induction l; eauto.
+  Qed.
+
+  (* Axiom about prims. Currently assuming that they do not return functions *)
+  Parameter primAxiom :
+    forall f f' vs v k,
+      M.get f pr = Some f' ->
+      f' vs = Some v ->
+      sizeOf_val k v = 0.
+
   (** Correctness of [Closure_conversion] *)
   Lemma Closure_conversion_correct k rho rho' e e' Scope Funs σ c Γ FVs C :
     (* [Scope] invariant *)
-    cc_approx_env_P pr cenv clo_tag Scope k rho rho' ->
+    cc_approx_env_P pr cenv clo_tag Scope k boundG rho rho' ->
     (* [Γ] (the current environment parameter) is not bound in e *)
     ~ In _ (bound_var e) Γ ->
     (* The free variables of e are defined in the environment *)
@@ -1560,7 +2224,7 @@ Section Closure_conversion_correct.
     FV_inv k rho rho' Scope Funs c Γ FVs ->
     (* [e'] is the closure conversion of [e] *)
     Closure_conversion clo_tag Scope Funs σ c Γ FVs e e' C ->
-    cc_approx_exp pr cenv clo_tag k (e, rho) (C |[ e' ]|, rho').
+    cc_approx_exp pr cenv clo_tag k (boundL k e rho) boundG (e, rho) (C |[ e' ]|, rho').
   Proof with now eauto with Ensembles_DB.
     revert k e rho rho' e' Scope Funs σ c Γ FVs C.
     induction k as [k IHk] using lt_wf_rec1.
@@ -1568,33 +2232,54 @@ Section Closure_conversion_correct.
       intros rho1 rho2 e' Scope Funs σ c' Γ FVs C Happrox Hnin HFVs Hun Hinj Hd Hfun Henv Hcc.
     - (* Case Econstr *)
       inv Hcc.
-      intros v1 c1 Hleq Hstep. inv Hstep.
-      edestruct project_vars_ctx_to_rho as [rho2' Hto_rho]; eauto.
-      edestruct project_vars_correct as [Happ [Hfun' [Henv' Hvar]]]; eauto.
-      eapply ctx_to_rho_cc_approx_exp; eauto.
-      edestruct Hvar as [v' [Hget' Happ']]; eauto. 
-      intros v1' c1' Hleq' Hstep'. eapply bstep_e_deterministic in H8; eauto. inv H8.
-      repeat normalize_bound_var_in_ctx.
-      edestruct IHe as [v2'' [c2 [Hstep2 Happrox2]]];
-        [| now eauto | | | eassumption | | | | eassumption | eassumption | eassumption | ]. 
-      + eapply cc_approx_env_P_extend with (v2 := Vconstr t v').
-        eapply cc_approx_env_P_antimon; [ eassumption |]...
-        rewrite cc_approx_val_eq. constructor; eauto.
-        now eapply Forall2_Forall2_asym_included.
-      + eapply binding_in_map_antimon; [| eapply binding_in_map_set; eassumption ].
-        eapply occurs_free_Econstr_Included. 
-      + intros f Hfin. eauto.
-      + eapply Disjoint_Included_r;
-        [| eapply Disjoint_Included_l; [ apply image_monotonic | now apply Hd ]]...
-      + eapply Fun_inv_set_In_Scope_l. now eauto.
-        eapply Fun_inv_set_In_Scope_r_not_Γ. now eauto.
-        intros Heq; subst. now eauto.
-        eapply Fun_inv_mon; [ | now eauto ]...
-      + eapply FV_inv_set_In_Scope_l. now constructor.
-        eapply FV_inv_set_r. intros Hc. eapply Hnin.
-        subst. now eauto. now eapply FV_inv_extend_Scope.
-      + repeat eexists; [| eassumption ].
-        econstructor; eauto.
+      assert(Hadm : sizeOf_exp_ctx C <= 3*length l) by (eapply project_vars_sizeOf_ctx_exp; eauto).
+      pose (P :=
+              fun n c1 c2 : nat =>
+                c1 + n <= c2 + sizeOf_exp_ctx C <= 7 * c1 * max_exp_env k e rho1
+                                                 + 7 * sizeOf_exp e + n).
+      eapply cc_approx_exp_rel_mon with (P1 := P (sizeOf_exp_ctx C)).
+      { intros v1 c1 Hleq Hstep. assert (Hstep' := Hstep). inv Hstep'.
+        edestruct project_vars_ctx_to_rho as [rho2' Hto_rho]; eauto.
+        edestruct project_vars_correct as [Happ [Hfun' [Henv' Hvar]]]; eauto.
+        edestruct Hvar as [v' [Hget' Happ']]; eauto.
+        eapply ctx_to_rho_cc_approx_exp with (P' := P 0); eauto.
+        - now firstorder.
+        - now firstorder.
+        - eapply cc_approx_exp_constr_compat with (S0 := boundL k e rho1).
+          + eapply Forall2_cc_approx_var_env; eauto.
+          + unfold boundL, upper_boundL, lower_boundL, P. intros c1 c2 n Hle.
+            rewrite <- !plus_n_O. intros [Hle1 Hle2]; split; try omega.
+            ring_simplify. rewrite <- !plus_assoc, (plus_comm c2).
+            eapply plus_le_compat; eauto. eapply plus_le_mult; eauto.
+            now apply max_exp_env_grt_1. eapply le_trans. eassumption.
+            omega.
+          + intros vs1 vs2 Hget Hall.
+            unfold boundL, upper_boundL, lower_boundL, max_exp_env.
+            erewrite <- sizeOf_env_set_constr; eauto.
+            eapply IHe; [ | | | | eassumption | | | | eassumption ].
+            * eapply cc_approx_env_P_extend with (v2 := Vconstr t vs2).
+              eapply cc_approx_env_P_antimon; [ eassumption |]...
+              rewrite cc_approx_val_eq. constructor; eauto.
+              now eapply Forall2_Forall2_asym_included.
+            * now eauto.
+            * eapply binding_in_map_antimon; [| eapply binding_in_map_set; eassumption ].
+              eapply occurs_free_Econstr_Included. 
+            * intros f Hfin. eauto.
+            * eapply Disjoint_Included_r;
+              [| eapply Disjoint_Included_l; [ apply image_monotonic | now apply Hd ]].
+              normalize_bound_var... now eauto with Ensembles_DB.
+            * eapply Fun_inv_set_In_Scope_l. now eauto.
+              eapply Fun_inv_set_In_Scope_r_not_Γ. now eauto.
+              intros Heq; subst. now eauto.
+              eapply Fun_inv_mon; [ | now eauto ]...
+            * eapply FV_inv_set_In_Scope_l. now constructor.
+              eapply FV_inv_set_r. intros Hc. eapply Hnin.
+              subst. now eauto. now eapply FV_inv_extend_Scope. }
+      { intros c1 c2. unfold P, boundL, lower_boundL, upper_boundL.
+        intros [Hle1 Hle2]; split; try omega.
+        eapply le_trans;
+          [| eapply plus_le_compat_r; eapply mult_le_compat_l; now apply max_exp_env_Econstr ].
+        simpl. omega. }
     - (* Case [Ecase x []] *)
       inv Hcc. inv H11.
       intros v1 c1 Hleq Hstep. inv Hstep. inv H5. 
@@ -1602,146 +2287,119 @@ Section Closure_conversion_correct.
       inv Hcc.
       inversion H11 as [ | [c1 p1] [c2 p2] l1 l2 [Heq [C' [e' [Heq' Hcc]]]] Hall ];
         simpl in Heq, Heq'; subst.
-      intros v1 c1 Hleq Hstep. inv Hstep.
       repeat normalize_bound_var_in_ctx.
-      simpl in H5. destruct (M.elt_eq c2 t) eqn:Heq; subst. 
-      { inv H3. inv H5. inv H8. 
-        - edestruct Happrox as [vcon [Hget' Happrox2]]; eauto.
-          rewrite cc_approx_val_eq in Happrox2.
-          destruct vcon; try contradiction. inv Happrox2.
-          edestruct IHe as [v2 [c2 [Hstep2 Happrox2]]];
-            [ eassumption
-            | now intros Hc; eapply Hnin; eauto | |
-            | eassumption | | eassumption | eassumption
-            | eassumption | eassumption | eassumption | ].
-          + eapply binding_in_map_antimon; [|  eassumption ].
-            eapply occurs_free_Ecase_Included. now constructor.
-          + intros f Hfin. eapply Hun.
-            econstructor. eassumption. now constructor. 
-          + eauto with Ensembles_DB.
-          + repeat eexists; [| eassumption ].
-            econstructor; eauto; [| simpl; now rewrite Heq ].
-            econstructor; eauto. inv H11. eapply caseConsistent_same_cTags.
-            eapply Forall2_monotonic; [| eassumption ].
-            intros x x2 H'. now inv H'. eassumption.
-        - edestruct Hfun as
-              [vs' [rho3 [B3 [f3 [rho4 [B4 [f4 [Hget1 [Heq2 [Ηnin2 [Hget2 Happrox']]]]]]]]]]]; eauto.
-          congruence.
-        - edestruct Henv as [vs2 [v' [Hget [Hnth' Happrox2]]]]; eauto.
-          rewrite cc_approx_val_eq in Happrox2.
-          destruct v'; try contradiction. inv Happrox2.
-          edestruct IHe as [v2 [c2 [Hstep2 Happrox2]]];
-            [| now intros Hc; eapply Hnin; eauto | | 
-             | eassumption | | | | eassumption | eassumption | eassumption
-             | ].
-          + eapply cc_approx_env_P_set_not_in_P_r. eassumption.
-            intros Hc. eapply H1. eauto.
-          + eapply binding_in_map_antimon; [|  eassumption ].
-            eapply occurs_free_Ecase_Included. now constructor.
-          + intros f Hfin. eapply Hun.
-            econstructor. eassumption. now constructor.
-          + eauto with Ensembles_DB.
-          + eapply Fun_inv_set_not_In_Funs_r_not_Γ; [| | eassumption ]. 
-            intros Hc. eapply H1. now eauto.
-            intros Heq'; subst. eapply H1. now eauto.
-          + eapply FV_inv_set_r. intros Hc. subst. eapply H1. now eauto.
-            eassumption.
-          +  repeat eexists; [| eassumption ]; econstructor; eauto.
-             econstructor; eauto;
-             [ rewrite M.gss ; reflexivity | | simpl; now rewrite Heq ].
-             inv H11. econstructor; eauto. eapply caseConsistent_same_cTags.
-             eapply Forall2_monotonic; [| eassumption ].
-             intros x x2 H'. now inv H'. eassumption. }
-      { inv H5. assert (H8' := H8). inv H8. 
-        - edestruct Happrox as [vcon [Hget' Happrox2]]; eauto.
-          rewrite cc_approx_val_eq in Happrox2.
-          destruct vcon; try contradiction. inv Happrox2.
-          edestruct IHe0 as [v2 [c2' [Hstep2 Happrox2]]];
-            [ eassumption
-            | now intros Hc; eapply Hnin; eauto | |
-            | eassumption | | eassumption | eassumption | now econstructor; eauto
-            | eassumption |  | ].
-          + eapply binding_in_map_antimon; [| eassumption ].
-            intros x Hin. inv Hin; eauto.
-          + intros f Hfin. eapply Hun. inv Hfin. 
-            econstructor; eauto. constructor 2. eassumption.
-          + eauto with Ensembles_DB.
-          + econstructor; eauto. inv H3. eassumption.
-          + inv Hstep2. repeat eexists; [| eassumption ].
-            inv H3.
-            econstructor; eauto. simpl. rewrite Hget' in H7. inv H7.
-            econstructor; eauto.
-            simpl. rewrite Hget' in H7. inv H7. now rewrite Heq.
-        -  edestruct Hfun as
-              [vs' [rho3 [B3 [f3 [rho4 [B4 [f4 [Hget1 [Heq2 [Ηnin2 [Hget2 Happrox']]]]]]]]]]]; eauto.
-          congruence.
-        - edestruct Henv as [vs2 [v' [Hget [Hnth' Happrox2]]]]; eauto.
-          rewrite cc_approx_val_eq in Happrox2.
-          destruct v'; try contradiction. inv Happrox2. inv H3.
-          edestruct IHe0 as [v2 [c2' [Hstep2 Happrox2]]];
-            [ eassumption
-            | now intros Hc; eapply Hnin; eauto | |
-            | eassumption | | eassumption | eassumption | now econstructor; eauto
-            | eassumption | now econstructor; eauto | ].
-          + eapply binding_in_map_antimon; [|  eassumption ].
-            intros x Hin. inv Hin; eauto.
-          + intros f Hfin. eapply Hun. inv Hfin.
-            econstructor; eauto. constructor 2. eassumption.
-          + eauto with Ensembles_DB.
-          + inv Hstep2; rewrite Hget in H20; inv H20; rewrite Hnth' in H21; inv H21.
-            inv H22. rewrite M.gss in H10. inv H10.
-            repeat eexists; [| eassumption ]; econstructor; eauto.
-            econstructor; eauto. simpl. rewrite M.gss; reflexivity.
-            now econstructor; eauto. simpl. now rewrite Heq. }
+      assert(Hadm : sizeOf_exp_ctx C <= 3) by (eapply project_var_sizeOf_ctx_exp; eauto).
+      intros v1 c1 Hleq Hstep. assert (Hstep' := Hstep). inv Hstep'.
+      edestruct project_var_ctx_to_rho as [rho2' Hto_rho]; eauto.
+      edestruct project_var_correct as [Happ [Hfun' [Henv' Hvar]]]; eauto.
+      edestruct Hvar as [Hget' Happ']; eauto. 
+      eapply Ecase_correct; try eassumption.
+      + inv H11. eapply Forall2_monotonic; try eassumption.
+        firstorder.
+      + eapply IHe; try eassumption.
+        * now intros Hc; eapply Hnin; eauto.
+        * eapply binding_in_map_antimon; [|  eassumption ].
+          eapply occurs_free_Ecase_Included. now constructor.
+        * intros f Hfin. eapply Hun.
+          econstructor. eassumption. now constructor.
+        * eauto with Ensembles_DB.
+      + eapply IHe0; try eassumption.
+        * now eauto.
+        * eapply binding_in_map_antimon; [| eassumption ].
+          intros x Hin. inv Hin; eauto.
+        * intros f Hfin. eapply Hun. inv Hfin. 
+          econstructor; eauto. constructor 2. eassumption.
+        * eauto with Ensembles_DB.
+        * econstructor; eauto.
     - (* Case Eproj *)
       inv Hcc.
-      intros v1 c1 Hleq Hstep. inv Hstep.
-      edestruct project_var_ctx_to_rho as [rho2' Hto_rho]; eauto.
-      edestruct project_var_correct as [Hnin' [Happ [Hfun' [Henv' Hvar]]]]; eauto.
-      edestruct Hvar as [v' [Hget' Happ']]; eauto.
-      rewrite cc_approx_val_eq in Happ'. destruct v'; try contradiction.
-      inv Happ'. eapply ctx_to_rho_cc_approx_exp; eauto.
-      intros v1' c1' Hleq' Hstep'. eapply bstep_e_deterministic in H9; eauto.
-      inv H9. edestruct (@Forall2_asym_nthN val) as [v2' [Hnth2 Happ2]]; eauto.
-      repeat normalize_bound_var_in_ctx.
-      edestruct IHe as [v2'' [c2 [Hstep2 Happrox2]]];
-        [| now eauto | | | eassumption | | |
-         | eassumption | eassumption | eassumption | ].
-      + eapply cc_approx_env_P_extend; [| eassumption ].
-        eapply cc_approx_env_P_antimon; [ eassumption |]...
-      + eapply binding_in_map_antimon; [| eapply binding_in_map_set; eassumption ].
-        eapply occurs_free_Eproj_Included. 
-      + intros f Hfin. eauto.
-      + eapply Disjoint_Included_r;
-        [| eapply Disjoint_Included_l; [ apply image_monotonic | now apply Hd ]]...
-      + eapply Fun_inv_set_In_Scope_l. now eauto.
-        eapply Fun_inv_set_In_Scope_r_not_Γ. now eauto.
-        intros Heq; subst. now eauto.
-        eapply Fun_inv_mon; [ | now eauto ]...
-      + eapply FV_inv_set_In_Scope_l. now constructor.
-        eapply FV_inv_set_r. intros Hc. eapply Hnin.
-        subst. now eauto. now eapply FV_inv_extend_Scope.
-      + repeat eexists; [| eassumption ]. econstructor; eauto. 
-    - (* Case Efun -- the hardest one! *) 
+      assert(Hadm : sizeOf_exp_ctx C <= 3) by (eapply project_var_sizeOf_ctx_exp; eauto).
+      pose (P :=
+              fun n c1 c2 : nat =>
+                c1 + n <= c2 + sizeOf_exp_ctx C <= 7 * c1 * max_exp_env k e rho1
+                                                 + 7 * sizeOf_exp e + n).
+      eapply cc_approx_exp_rel_mon with (P1 := P (sizeOf_exp_ctx C)).
+      { intros v1 c1 Hleq Hstep. assert (Hstep' := Hstep). inv Hstep'.
+        edestruct project_var_ctx_to_rho as [rho2' Hto_rho]; eauto.
+        edestruct project_var_correct as [Happ [Hfun' [Henv' Hvar]]]; eauto.
+        edestruct Hvar as [Hget' Happ']; eauto.
+        eapply ctx_to_rho_cc_approx_exp with (P' := P 0); eauto.
+        - now firstorder.
+        - now firstorder.
+        - eapply cc_approx_exp_proj_compat with (S0 := boundL k e rho1).
+          + eassumption.
+          + unfold boundL, upper_boundL, lower_boundL, P. intros c1 c2.
+            rewrite <- !plus_n_O. intros [Hle1 Hle2]; split; try omega.
+            ring_simplify. rewrite <- !plus_assoc.
+            rewrite (plus_comm _ (7 * _)), (plus_assoc _ (7 * _)).
+            eapply plus_le_compat; eauto.
+            eapply le_trans with (m := 4). omega.
+            specialize (max_exp_env_grt_1 k e rho1). omega.
+          + intros v1' v2' c1 vs1 Hget Hin Hv.
+            unfold boundL, lower_boundL, upper_boundL, max_exp_env.
+            erewrite <- sizeOf_env_set_proj; eauto.
+            eapply IHe; [ | | | | eassumption | | | | eassumption ].
+            * eapply cc_approx_env_P_extend.
+              eapply cc_approx_env_P_antimon; [ eassumption |]...
+              eassumption.
+            * now eauto.
+            * eapply binding_in_map_antimon; [| eapply binding_in_map_set; eassumption ].
+              eapply occurs_free_Eproj_Included. 
+            * intros f Hfin. eauto.
+            * eapply Disjoint_Included_r;
+              [| eapply Disjoint_Included_l; [ apply image_monotonic | now apply Hd ]].
+              normalize_bound_var... now eauto with Ensembles_DB.
+            * eapply Fun_inv_set_In_Scope_l. now eauto.
+              eapply Fun_inv_set_In_Scope_r_not_Γ. now eauto.
+              intros Heq; subst. now eauto.
+              eapply Fun_inv_mon; [ | now eauto ]...
+            * eapply FV_inv_set_In_Scope_l. now constructor.
+              eapply FV_inv_set_r. intros Hc. eapply Hnin.
+              subst. now eauto. now eapply FV_inv_extend_Scope. }
+      { intros c1 c2. unfold P, boundL, lower_boundL, upper_boundL.
+        intros [Hle1 Hle2]; split; try omega.
+        eapply le_trans; [| eapply plus_le_compat_r; eapply mult_le_compat_l; now apply max_exp_env_Eproj ].
+        simpl. omega. }
+    - (* Case Efun -- the hardest one! *)
       inv Hcc.
+      specialize (occurs_free_fundefs_cardinality _ _ (proj2 H1) H2); intros Hlen.
       assert (Ha : exists vs, getlist FVs' rho1 = Some vs).
-      { eapply In_getlist. intros x Hin. eapply HFVs. 
+      { eapply In_getlist. intros x Hin. eapply HFVs.
         rewrite occurs_free_Efun, H1. eauto. }
       destruct Ha as [vs Hgetlist].
+      (* sizes of evaluation contexts *)
+      assert(HC1 : sizeOf_exp_ctx C' <= 3 * sizeOf_fundefs f2)
+        by (eapply le_trans; [ now eapply project_vars_sizeOf_ctx_exp; eauto | omega ]).
+      assert (HC2 : sizeOf_exp_ctx C0 <= 3 * numOf_fundefs f2)
+        by (eapply make_closures_sizeOf_ctx_exp; eauto).
+      pose (P1 :=
+              fun m n c1 c2 : nat => 
+                c1 + n <= c2 + sizeOf_exp_ctx C' <= 7 * c1 * max_exp_env k (Efun f2 e) rho1
+                                                  + m * sizeOf_fundefs f2 + 7 * sizeOf_exp e + 7
+                                                  + n).
+      pose (P2 :=
+              fun m n c1 c2 : nat => 
+                c1 + n <= c2 + sizeOf_exp_ctx C0 <= 7 * c1 * max_exp_env k (Efun f2 e) rho1
+                                                  + m * sizeOf_fundefs f2 + 7 * sizeOf_exp e + 6
+                                                  + n).
+      eapply cc_approx_exp_rel_mon with (P1 := P1 7 (sizeOf_exp_ctx C'));
+        [| intros c1 c2; unfold P1, boundL, lower_boundL, upper_boundL;
+           intros [Hle1 Hle2]; split; simpl; omega ].
       intros v1 c1 Hleq Hstep.
       edestruct project_vars_ctx_to_rho as [rho2' Hto_rho]; [ | eassumption | | | | ]; eauto.
       edestruct project_vars_correct as [Happ [Hfun' [Henv' Hvar]]]; eauto.
-      edestruct Hvar as [v' [Hget' Happ']]; eauto. rewrite <- app_ctx_f_fuse.
-      eapply ctx_to_rho_cc_approx_exp; eauto.
-      repeat normalize_bound_var_in_ctx.
+      edestruct Hvar as [v' [Hget' Happ']]; eauto. rewrite <- app_ctx_f_fuse. simpl.
+      eapply ctx_to_rho_cc_approx_exp with (P' := P1 7 0);
+        try eassumption;
+        try now (intros n1 n2; unfold P1; intros; simpl; omega).
       assert (Hsuf :
-                cc_approx_exp pr cenv clo_tag k (e, def_funs f2 f2 rho1 rho1)
+                cc_approx_exp pr cenv clo_tag k (P2 3 (sizeOf_exp_ctx C0))  boundG (e, def_funs f2 f2 rho1 rho1)
                               (C0 |[ Ce |[ e'0 ]| ]|, def_funs B' B' (M.set Γ' (Vconstr c'0 v') rho2')
                                                    (M.set Γ' (Vconstr c'0 v') rho2'))).
       { edestruct make_closures_ctx_to_rho as [rho2'' Htp_rho']; eauto.
         - eapply Disjoint_Included_r; [| eassumption ].
           apply Included_Union_preserv_l. now apply name_in_fundefs_bound_var_fundefs.
-        - intros Hc. eapply H4. now eauto.
+        - intros Hc. eapply H5. now eauto.
         - eapply Closure_conversion_fundefs_correct; eauto. 
           + intros f Hfin. inv Hfin; eauto.
           + intros f Hfin. inv Hfin; eauto.
@@ -1758,13 +2416,13 @@ Section Closure_conversion_correct.
           + eapply make_closures_injective; [| eassumption ].
             eapply Disjoint_Included_r; [| eassumption ].
             apply Included_Union_preserv_l. now apply name_in_fundefs_bound_var_fundefs.
-          + intros Hc. eapply H4. now eauto.
-          + intros Hc. eapply H4. now eauto.
+          + intros Hc. eapply H5. now eauto.
+          + intros Hc. eapply H5. now eauto.
           + intros Hc. erewrite <- closure_conversion_fundefs_Same_set_image in Hc; [| eassumption ].
-            eapply H6. constructor; [| now eauto ].
+            eapply H7. constructor; [| now eauto ].
             eapply make_closures_image_Included. eassumption. eassumption.
           + intros Hc. erewrite <- closure_conversion_fundefs_Same_set_image in Hc; [| eassumption ].
-            eapply H6. constructor; [| now eauto ].
+            eapply H7. constructor; [| now eauto ].
             eapply make_closures_image_Included. eassumption. eassumption.
           + edestruct Hvar as [vs' [Hgetlist' Hall]]; eauto.
             intros x N v _ _ Hnth Hget. rewrite Hget' in Hgetlist'; inv Hgetlist'.
@@ -1784,7 +2442,7 @@ Section Closure_conversion_correct.
           + eauto.
           + intros Hc. eapply Hnin. constructor.
             now eapply name_in_fundefs_bound_var_fundefs.
-          + intros Hc. eapply H4. now eauto.
+          + intros Hc. eapply H5. now eauto.
           + eapply Included_Union_l.
           + eapply Disjoint_Included_r; [| eassumption ].
             apply Included_Union_preserv_l. now apply name_in_fundefs_bound_var_fundefs.
@@ -1797,10 +2455,10 @@ Section Closure_conversion_correct.
             now eauto 7 with Ensembles_DB.
             eapply cc_approx_env_P_set_not_in_P_r.
             eapply cc_approx_env_P_antimon; [ eassumption |]...
-            intros Hin. inv Hin. inv H. eauto. eapply H4. eauto.
-          + eapply Fun_inv_def_funs.
+            intros Hin. inv Hin. inv H. eauto. eapply H5. eauto.
+          + repeat normalize_bound_var_in_ctx. eapply Fun_inv_def_funs.
             * intros Hc. erewrite <- closure_conversion_fundefs_Same_set_image in Hc; [| eassumption ].
-              eapply H6. constructor.
+              eapply H7. constructor.
               eapply make_closures_image_Included. eassumption. eassumption.
               rewrite !Union_assoc...
             * intros Hc. eapply Hnin. eapply Included_Union_l.
@@ -1811,20 +2469,19 @@ Section Closure_conversion_correct.
               eapply Disjoint_Included_r;
                 [ eapply make_closures_image_Included; eassumption |]...
             * eapply Fun_inv_set_not_In_Funs_r_not_Γ; [| | ].
-              intros Hc. eapply H4. now eauto.
-              intros Hc. subst. eapply H4. constructor. now eauto.
+              intros Hc. eapply H5. now eauto.
+              intros Hc. subst. eapply H5. constructor. now eauto.
               now eauto. now eauto.
           + eapply FV_inv_def_funs.
             * intros Hc. eapply Hnin. constructor. 
               now eapply name_in_fundefs_bound_var_fundefs.
             * intros Hc.
               erewrite <- closure_conversion_fundefs_Same_set_image in Hc; [| eassumption ].
-              eapply H6. constructor.
+              eapply H7. constructor.
               eapply make_closures_image_Included. eassumption. eassumption.
               rewrite !Union_assoc. now apply Included_Union_r.
             * eapply  FV_inv_set_r.
-              intros Hc. subst. eapply H4. constructor; eauto.
-              eassumption. 
+              intros Hc. subst. eapply H5. constructor; eauto. eassumption. 
           + eapply Closure_conversion_fundefs_correct with (c := c'0) ; eauto.
             * intros f Hfin. inv Hfin; eauto.
             * intros f Hfin. inv Hfin; eauto.
@@ -1840,14 +2497,14 @@ Section Closure_conversion_correct.
             * eapply make_closures_injective; [| eassumption].
               eapply Disjoint_Included_r; [| eassumption ].
               apply Included_Union_preserv_l. now apply name_in_fundefs_bound_var_fundefs.
-            * intros Hc. eapply H4. now eauto.
-            * intros Hc. eapply H4. now eauto.
+            * intros Hc. eapply H5. now eauto.
+            * intros Hc. eapply H5. now eauto.
             * intros Hc. erewrite <- closure_conversion_fundefs_Same_set_image in Hc; [| eassumption ].     
-              eapply H6. constructor.
+              eapply H7. constructor.
               eapply make_closures_image_Included. eassumption.
               eassumption. now eauto.
             * intros Hc. erewrite <- closure_conversion_fundefs_Same_set_image in Hc; [| eassumption ].     
-              eapply H6. constructor.
+              eapply H7. constructor.
               eapply make_closures_image_Included. eassumption.
               eassumption. now eauto.
             * edestruct Hvar as [vs' [Hgetlist' Hall]]; eauto.
@@ -1857,93 +2514,188 @@ Section Closure_conversion_correct.
               edestruct (@Forall2_nthN val) as [v'' [Hget''' Hcc'']]. eassumption.
               eassumption. rewrite Hget in Hget''. inv Hget''. eauto.
           + eauto.
-          + eapply ctx_to_rho_cc_approx_exp; eauto.
-            eapply IHe; eauto. 
+          + eapply ctx_to_rho_cc_approx_exp with (P' := P2 3 0);
+            try eassumption;
+            try now (intros n1 n2; unfold P2; intros; simpl; omega).
+            eapply cc_approx_exp_rel_mon; [ eapply IHe; eauto |].
             * eapply binding_in_map_antimon.
               eapply Included_trans. now eapply occurs_free_Efun_Included.
               rewrite Union_commut. now apply Included_refl.
               apply binding_in_map_def_funs. eassumption.
-            * intros f Hfin; eauto.
-            * eapply Disjoint_Included_r;
+            * intros f Hfin; eauto. 
+            * repeat normalize_bound_var_in_ctx.
+              eapply Disjoint_Included_r;
               [| eapply Disjoint_Included_l;
-                 [ apply image_monotonic | now apply Hd ]]... }
+                 [ apply image_monotonic | now apply Hd ]]...
+            * intros n1 n2; unfold boundL, lower_boundL, upper_boundL, P2.
+              rewrite <- !plus_n_O. intros [Hle1 Hle2]; split; try omega.
+              eapply le_trans. eapply plus_le_compat. eassumption.
+              eapply le_trans. eassumption. eapply mult_le_compat_l.
+              now apply numOf_fundefs_le_sizeOf_fundefs.
+              eapply le_trans. do 2 eapply plus_le_compat_r.
+              eapply mult_le_compat_l. now eapply max_exp_env_Efun.
+              omega. }
       intros v1' c1' Hleq' Hstep'. inv Hstep'.
-      edestruct Hsuf as [v2' [c2' [Hstep2' Hcc2']]]; [| eassumption |]; eauto.
-      repeat eexists; eauto. econstructor; eauto. econstructor; eauto.
+      edestruct Hsuf as [v2' [c2' [Hstep2' [[Hle1 Hle2] Hcc2']]]]; [| eassumption |]; eauto.
+      assert (Hadm : length FVs' = length FVs'').
+      {  do 2 (erewrite getlist_length_eq; [| eassumption ]).
+         eapply Forall2_length. eassumption. }
+      assert (Hadm' : numOf_fundefs f2 = numOf_fundefs B')
+        by (eapply Closure_conversion_fundefs_numOf_fundefs; eauto).
+      do 2 eexists. split; [| split ].
+      econstructor; eauto. econstructor; eauto.
+      unfold P1 in Hle1, Hle2. split; omega.
+      eapply cc_approx_val_monotonic; try eassumption. omega.
     - (* Case Eapp *)
       inv Hcc.
-      intros v1 c1 Hleq Hstep. inv Hstep.
-      edestruct project_vars_ctx_to_rho as [rho2' Hto_rho]; eauto.
-      simpl. rewrite H4, H5. reflexivity.
-      edestruct project_vars_correct as [Happ [Hfun' [Henv' Hvar]]]; eauto.
-      edestruct Hvar as [v' [Hget' Happ']]; eauto.
-      simpl. rewrite H4, H5. reflexivity.
-      simpl in Hget'. destruct (M.get f' rho2') eqn:Hgetf'; try discriminate.
-      destruct (getlist ys' rho2') eqn:Hgetlist'; try discriminate. inv Hget'.
-      inv Happ'. rewrite cc_approx_val_eq in H6. destruct v0; try contradiction.
-      eapply ctx_to_rho_cc_approx_exp with (e := Eapp v t l); eauto.
-      * intros v1' c1' Hleq' Hstep'. inv Hstep'.
+      assert(Hadm : sizeOf_exp_ctx C <= 3 * length l + 3)
+        by (eapply le_trans; [ now eapply project_vars_sizeOf_ctx_exp; eauto | simpl; omega ]).
+      pose (P :=
+              fun n c1 c2 : nat =>
+                c1 + n <= c2 + sizeOf_exp_ctx C <= 7 * c1 * max_exp_env k (Eapp v t l) rho1
+                                                 + 7 * sizeOf_exp (Eapp v t l) 
+                                                 + n).
+      eapply cc_approx_exp_rel_mon with (P1 := P (sizeOf_exp_ctx C));
+        [| intros n1 n2; unfold P, boundL, upper_boundL, lower_boundL; simpl; omega ].
+      { intros v1 c1 Hleq Hstep. assert (Hstep' := Hstep); inv Hstep'.
+        edestruct project_vars_ctx_to_rho as [rho2' Hto_rho]; eauto.
+        simpl. rewrite H4, H5. reflexivity.
+        edestruct project_vars_correct as [Happ [Hfun' [Henv' Hvar]]]; eauto.
+        edestruct Hvar as [v' [Hget' Happ']]; eauto.
+        simpl. rewrite H4, H5. reflexivity.
+        simpl in Hget'. destruct (M.get f' rho2') eqn:Hgetf'; try discriminate.
+        destruct (getlist ys' rho2') eqn:Hgetlist'; try discriminate. inv Hget'.
+        inv Happ'. rewrite cc_approx_val_eq in H6. destruct v0; try contradiction.
+        eapply ctx_to_rho_cc_approx_exp with (P' := P 0);
+          [ now firstorder
+          | now (intros n1 n2; simpl; unfold P; intros; omega) | | | | ]; try eassumption.
+        intros v1' c1' Hleq' Hstep'. inv Hstep'.
         rewrite H4 in H8. inv H8. rewrite H5 in H15; inv H15.
         destruct l1; try contradiction. destruct v0, l1; try contradiction.
-        destruct v2; try contradiction.
+        destruct v2; try contradiction. 
         rewrite H17 in H7. inv H7. 
-        rewrite H11 in H20. inv H20. eapply bstep_e_deterministic in H21; eauto. inv H21.
+        rewrite H11 in H20. inv H20. eapply bstep_cost_deterministic in H21; eauto. inv H21.
         assert (Hlen := List_util.Forall2_length _ _ _ H9).
         edestruct H6 with (vs2 := l0) (j := k - 1)
           as [Γ' [xs2 [e2 [rho2'' [Heq [Hfind [Hset Hyp]]]]]]]; eauto.
-        edestruct Hyp as [v2' [c'2 [Hstep2 Hcc']]]; try eassumption. omega.
-        eapply List_util.Forall2_monotonic; [| eassumption ].
-        intros. eapply cc_approx_val_monotonic. eassumption. omega. omega.
-        subst. repeat eexists. econstructor. eassumption. reflexivity.
-        econstructor. rewrite M.gso. eassumption.
-        intros Hc; subst. eapply project_vars_not_In_free_set; [ now eauto | now eauto | ].
-        constructor. now eapply H10. rewrite FromList_cons. now eauto.
-        reflexivity.
-        eapply BStep_app. rewrite M.gso. rewrite M.gss. reflexivity.
-        now eauto.
-        simpl. rewrite M.gss. rewrite getlist_set_neq. rewrite getlist_set_neq.
-        rewrite Hgetlist'. reflexivity. 
-        intros Hin. eapply project_vars_not_In_free_set. eassumption. eassumption. 
-        constructor. eapply H10. rewrite FromList_cons. now eauto.
-        intros Hin. eapply project_vars_not_In_free_set. eassumption. eassumption.
-        constructor. now eauto. rewrite FromList_cons. now eauto.
-        eassumption. simpl in Hset. eauto. eassumption.
-        eapply cc_approx_val_monotonic. eassumption. omega.
-      * econstructor; eauto.
+        edestruct Hyp as [v2' [c'2 [Hstep2 [[Hle1 Hle2] Hcc']]]]; try eassumption.
+        - omega.
+        - eapply List_util.Forall2_monotonic; [| eassumption ].
+          intros. eapply cc_approx_val_monotonic. eassumption. omega.
+        - omega.
+        - subst.
+          assert (Heq: length ys' = length l).
+          { symmetry. do 2 (erewrite getlist_length_eq; [| eassumption ]).
+            eapply Forall2_length. eassumption. }
+          repeat eexists.
+          + econstructor. eassumption. reflexivity.
+            econstructor. rewrite M.gso. eassumption.
+            intros Hc; subst. eapply project_vars_not_In_free_set; [ now eauto | now eauto | ].
+            constructor. now eapply H10. rewrite FromList_cons. now eauto.
+            reflexivity.
+            eapply BStepc_app. rewrite M.gso. rewrite M.gss. reflexivity.
+            now eauto.
+            simpl. rewrite M.gss. rewrite getlist_set_neq. rewrite getlist_set_neq.
+            rewrite Hgetlist'. reflexivity. 
+            intros Hin. eapply project_vars_not_In_free_set. eassumption. eassumption. 
+            constructor. eapply H10. rewrite FromList_cons. now eauto.
+            intros Hin. eapply project_vars_not_In_free_set. eassumption. eassumption.
+            constructor. now eauto. rewrite FromList_cons. now eauto.
+            eassumption. simpl in Hset. eauto. eassumption. 
+          + simpl. unfold boundG, boundL, upper_boundL, lower_boundL in Hle1.
+            omega.
+          + unfold boundG, boundL, upper_boundL, lower_boundL in Hle2.
+            assert (Hles : sizeOf_exp e <= sizeOf_env k rho1).
+            { eapply le_trans; [| now eapply sizeOf_env_get; eauto ].
+              destruct k; try omega. simpl. eapply le_trans. 
+              eapply fun_in_fundefs_sizeOf_exp; eauto. now eapply find_def_correct; eauto.
+              now apply Max.le_max_l. }
+            rewrite <- ! plus_assoc. rewrite <- plus_n_O.
+            eapply plus_le_compat; [| simpl; omega ].
+            rewrite <- mult_assoc, NPeano.Nat.mul_add_distr_r, NPeano.Nat.mul_add_distr_l.
+            eapply le_trans. eassumption. eapply plus_le_compat.
+            { destruct (Nat.eq_0_gt_0_cases k); subst.
+              * unfold max_exp_env. rewrite sizeOf_env_O, Max.max_0_r.
+                rewrite mult_assoc. eapply mult_le_compat_l.
+                eapply le_trans. eassumption. now apply Max.le_max_r.
+              * eapply le_trans. eapply mult_le_compat_l.
+                eapply sizeOf_env_set_app; eauto.
+                eapply fun_in_fundefs_sizeOf_exp; eauto. now eapply find_def_correct; eauto.
+                rewrite mult_assoc. eapply mult_le_compat_l. now apply Max.le_max_r. }
+            { rewrite mult_assoc. eapply mult_le_compat. omega.
+              eapply le_trans; [eassumption |  now apply Max.le_max_r ]. }
+          + eapply cc_approx_val_monotonic. eassumption. omega. }
     (* Case Eprim *)
     - inv Hcc.
-      intros v1 c1 Hleq Hstep. inv Hstep.
-      edestruct project_vars_ctx_to_rho as [rho2' Hto_rho]; eauto.
-      edestruct project_vars_correct as [Happ [Hfun' [Henv' Hvar]]]; eauto.
-      edestruct Hvar as [v' [Hget' Happ']]; eauto.
-      eapply ctx_to_rho_cc_approx_exp; eauto.
-      intros v1' c1' Hleq' Hstep'. eapply bstep_e_deterministic in H10; eauto.
-      inv H10. edestruct Prim_axiom_cc as [vs' [Hf' Hcc]]; eauto.
-      repeat normalize_bound_var_in_ctx.
-      edestruct IHe as [v2'' [c2 [Hstep2 Happrox2]]];
-        [| now eauto | | | eassumption | | | | eassumption | eassumption | eassumption | ]. 
-      + eapply cc_approx_env_P_extend; [| eassumption ].
-        eapply cc_approx_env_P_antimon; [ eassumption |]...
-      + eapply binding_in_map_antimon; [| eapply binding_in_map_set; eassumption ].
-        eapply occurs_free_Eprim_Included. 
-      + intros f Hfin. eauto.
-      + eapply Disjoint_Included_r;
-        [| eapply Disjoint_Included_l; [ apply image_monotonic | now apply Hd ]]...
-      + eapply Fun_inv_set_In_Scope_l. now eauto.
-        eapply Fun_inv_set_In_Scope_r_not_Γ. now eauto.
-        intros Heq; subst. now eauto.
-        eapply Fun_inv_mon; [ | now eauto ]...
-      + eapply FV_inv_set_In_Scope_l. now constructor.
-        eapply FV_inv_set_r. intros Hc. eapply Hnin.
-        subst. now eauto. now eapply FV_inv_extend_Scope.
-      + repeat eexists; [| eassumption ]. econstructor; eauto.
+      assert(Hadm : sizeOf_exp_ctx C <= 3*length l) by (eapply project_vars_sizeOf_ctx_exp; eauto).
+      pose (P :=
+              fun n c1 c2 : nat =>
+                c1 + n <= c2 + sizeOf_exp_ctx C <= 7 * c1 * max_exp_env k e rho1
+                                                 + 7 * sizeOf_exp e + n).
+      eapply cc_approx_exp_rel_mon with (P1 := P (sizeOf_exp_ctx C)).
+      { intros v1 c1 Hleq Hstep. assert (Hstep' := Hstep). inv Hstep'.
+        edestruct project_vars_ctx_to_rho as [rho2' Hto_rho]; eauto.
+        edestruct project_vars_correct as [Happ [Hfun' [Henv' Hvar]]]; eauto.
+        edestruct Hvar as [v' [Hget' Happ']]; eauto.
+        eapply ctx_to_rho_cc_approx_exp with (P' := P 0); eauto.
+        - now firstorder.
+        - now firstorder.
+        - eapply cc_approx_exp_prim_compat with (S0 := boundL k e rho1).
+          + unfold boundL, upper_boundL, lower_boundL, P. intros c1 c2 n Hle.
+            rewrite <- !plus_n_O. intros [Hle1 Hle2]; split; try omega.
+            ring_simplify. rewrite <- !plus_assoc, (plus_comm c2).
+            eapply plus_le_compat; eauto. eapply plus_le_mult; eauto.
+            now apply max_exp_env_grt_1. eapply le_trans. eassumption.
+            omega.
+          + eapply Forall2_cc_approx_var_env; eauto.
+          + intros vs1 vs2 l1 f Hgetl Hgetf Happf Hall.
+            unfold boundL, upper_boundL, lower_boundL, max_exp_env.
+            assert (HadmX : sizeOf_env k rho1 = sizeOf_env k (M.set  v vs1 rho1)).
+            { erewrite sizeOf_env_set, primAxiom; eauto. }
+            erewrite HadmX; eauto.
+            eapply IHe; [ | | | | eassumption | | | | eassumption ].
+            * eapply cc_approx_env_P_extend with (v2 := vs2).
+              eapply cc_approx_env_P_antimon; [ eassumption |]...
+              eassumption.
+            * now eauto.
+            * eapply binding_in_map_antimon; [| eapply binding_in_map_set; eassumption ].
+              eapply occurs_free_Eprim_Included. 
+            * intros f1 Hfin. eauto.
+            * eapply Disjoint_Included_r;
+              [| eapply Disjoint_Included_l; [ apply image_monotonic | now apply Hd ]].
+              normalize_bound_var... now eauto with Ensembles_DB.
+            * eapply Fun_inv_set_In_Scope_l. now eauto.
+              eapply Fun_inv_set_In_Scope_r_not_Γ. now eauto.
+              intros Heq; subst. now eauto.
+              eapply Fun_inv_mon; [ | now eauto ]...
+            * eapply FV_inv_set_In_Scope_l. now constructor.
+              eapply FV_inv_set_r. intros Hc. eapply Hnin.
+              subst. now eauto. now eapply FV_inv_extend_Scope. }
+      { intros c1 c2. unfold P, boundL, lower_boundL, upper_boundL.
+        intros [Hle1 Hle2]; split; try omega.
+        eapply le_trans;
+          [| eapply plus_le_compat_r; eapply mult_le_compat_l; now apply max_exp_env_Eprim ].
+        simpl. omega. }
+   (* Case Ehalt *)
     - inv Hcc.
-      intros v1 c1 Hleq Hstep. inv Hstep.
-      edestruct project_var_ctx_to_rho as [rho2' Hto_rho]; eauto.
-      edestruct project_var_correct as [Hnin' [Happ [Hfun' [Henv' Hvar]]]]; eauto.
-      edestruct Hvar as [v' [Hget' Happ']]; eauto.
-      eapply ctx_to_rho_cc_approx_exp; eauto.
-      eapply cc_approx_exp_halt_compat. eassumption. now econstructor; eauto.
+      assert(Hadm : sizeOf_exp_ctx C <= 3) by (eapply project_var_sizeOf_ctx_exp; eauto).
+      pose (P :=
+              fun n c1 c2 : nat =>
+                c1 + n <= c2 + sizeOf_exp_ctx C <= 7 * c1 * max_exp_env k (Ehalt v) rho1
+                                                 + 7 + n).
+      eapply cc_approx_exp_rel_mon with (P1 := P (sizeOf_exp_ctx C)).
+      { intros v1 c1 Hleq Hstep. assert (Hstep' := Hstep). inv Hstep'.
+        edestruct project_var_ctx_to_rho as [rho2' Hto_rho]; eauto.
+        edestruct project_var_correct as [Hnin' [Happ [Hfun' [Henv' Hvar]]]]; eauto.
+        edestruct Hvar as [v' [Hget' Happ']]; eauto.
+        eapply ctx_to_rho_cc_approx_exp with (P' := P 0); eauto.
+        - now firstorder.
+        - now firstorder.
+        - eapply cc_approx_exp_halt_compat.
+          unfold P. omega.
+          eassumption. }
+      { intros c1 c2. unfold P, boundL, lower_boundL, upper_boundL.
+        intros [Hle1 Hle2]; split; try simpl; omega. }
   Qed.
-
+  
 End Closure_conversion_correct. 
